update

theories/System/Regex.v
@@ -12,29 +12,30 @@ Inductive t {A : Type} : Type :=
 
 #[global] Arguments t : clear implicits.
 
-Inductive regex_semantics {A : Type} : Re.t A -> list A -> Prop :=
-  | rs_Empty
-    : regex_semantics (Empty) []
-  | rs_Char c
-    : regex_semantics (Char c) [c]
-  | rs_Union_l s e1 e2
-    (H_inl : regex_semantics e1 s)
-    : regex_semantics (Union e1 e2) s
-  | rs_Union_r s e1 e2
-    (H_inr : regex_semantics e2 s)
-    : regex_semantics (Union e1 e2) s
-  | rs_Append s1 s2 e1 e2
-    (H_in1 : regex_semantics e1 s1)
-    (H_in2 : regex_semantics e2 s2)
-    : regex_semantics (Append e1 e2) (s1 ++ s2)
-  | rs_Star_nil e1
-    : regex_semantics (Star e1) []
-  | rs_Star_app e1 s1 s2
-    (H_in1 : regex_semantics e1 s1)
-    (H_in2 : regex_semantics (Star e1) s2)
-    : regex_semantics (Star e1) (s1 ++ s2).
+Inductive in_regex {A : Type} : Re.t A -> list A -> Prop :=
+  | in_Empty
+    : [] ∈ Empty
+  | in_Char c
+    : [c] ∈ Char c
+  | in_Union_l s e1 e2
+    (H_inl : s ∈ e1)
+    : s ∈ Union e1 e2
+  | in_Union_r s e1 e2
+    (H_inr : s ∈ e2)
+    : s ∈ Union e1 e2
+  | in_Append s1 s2 e1 e2
+    (H_in1 : s1 ∈ e1)
+    (H_in2 : s2 ∈ e2)
+    : s1 ++ s2 ∈ Append e1 e2
+  | in_Star_nil e1
+    : [] ∈ Star e1
+  | in_Star_app e1 s1 s2
+    (H_in1 : s1 ∈ e1)
+    (H_in2 : s2 ∈ Star e1)
+    : s1 ++ s2 ∈ Star e1
+  where "s ∈ e" := (in_regex e s).
 
-#[global] Hint Constructors regex_semantics : simplication_hints.
+#[global] Hint Constructors in_regex : simplication_hints.
 
 End Re.
 
@@ -50,7 +51,6 @@ Section LANGUAGE.
 #[local] Opaque liftM2.
 
 Import Re.
-Import ListNotations.
 
 Context {A : Type}.
 
@@ -78,7 +78,7 @@ Fixpoint eval_regex (e : regex A) {struct e} : lang :=
   end.
 
 Theorem eval_regex_good e s
-  : s \in eval_regex e <-> regex_semantics e s.
+  : s \in eval_regex e <-> s ∈ e.
 Proof with eauto with *.
   split.
   - revert s; induction e; simpl; intros s H_IN; rewrite!; subst...
@@ -86,6 +86,134 @@ Proof with eauto with *.
     + des; subst...
     + induction H_IN...
   - intros H_in; induction H_in; simpl; rewrite!...
+Qed.
+
+Fixpoint fromString (s : list A) : regex A :=
+  match s with
+  | [] => Empty
+  | c :: s => Append (Char c) (fromString s)
+  end.
+
+Lemma fromString_spec (s : list A)
+  : eval_regex (fromString s) == E.singleton s.
+Proof with eauto with *.
+  induction s as [ | c s IH]; simpl... intros xs; (do 3 red in IH); rewrite!; split.
+  - intros ?; des. subst xs. rewrite!. rewrite IH in H0. rewrite!. subst...
+  - intros ->. exists [c]; rewrite!; split... exists s; split... rewrite IH; rewrite!...
+Qed.
+
+Fixpoint pow (s : list A) (n : nat) {struct n} : list A :=
+  match n with
+  | O => []
+  | S n' => s ++ s ^ n'
+  end
+where " s ^ n " := (pow s n) : list_scope.
+
+Lemma pow_in_star (s : list A) (e : regex A)
+  (s_in_e : s ∈ e)
+  : forall n : nat, s ^ n ∈ Star e.
+Proof.
+  induction n as [ | n IH]; simpl; eauto with *.
+Qed.
+
+Lemma pow_concat (n1 : nat) (n2 : nat) (s : list A)
+  : s ^ (n1 + n2) = s ^ n1 ++ s ^ n2.
+Proof.
+  revert n2 s. induction n1 as [ | n1 IH]; simpl; eauto.
+  ii. rewrite <- app_assoc. rewrite IH; eauto.
+Qed.
+
+Lemma pow_star (n : nat) (s1 : list A) (s2 : list A) (e : regex A)
+  (H_in1 : s1 ∈ e)
+  (H_in2 : s2 ∈ Star e)
+  : s1 ^ n ++ s2 ∈ Star e.
+Proof.
+  revert s1 s2 e H_in1 H_in2. induction n as [ | n IH]; simpl; eauto.
+  ii. rewrite <- app_assoc; eauto with *.
+Qed.
+
+Lemma star1 (s : list A) (e : regex A)
+  (H_in : s ∈ e)
+  : s ∈ Star e.
+Proof.
+  rewrite <- eval_regex_good; simpl.
+  rewrite <- app_nil_r with (l := s).
+  econstructor; eauto with *.
+  rewrite -> eval_regex_good; trivial.
+Qed.
+
+Fixpoint pumping_constant (e : regex A) : nat :=
+  match e with
+  | Null => 1
+  | Empty => 1
+  | Char c => 2
+  | Union e1 e2 => pumping_constant e1 + pumping_constant e2
+  | Append e1 e2 => pumping_constant e1 + pumping_constant e2
+  | Star e1 => pumping_constant e1
+  end.
+
+Lemma pumping_constant_ge_1 (e : regex A)
+  : pumping_constant e >= 1.
+Proof.
+  induction e; simpl; lia.
+Qed.
+
+Variant PUMPING_spec (e : regex A) (s : list A) : Prop :=
+  | PUMPING_spec_intro (s1 : list A) (s2 : list A) (s3 : list A)
+    (H_split : s = s1 ++ s2 ++ s3)
+    (H_ne_nil : s2 <> [])
+    (H_constant_ge : length s1 + length s2 <= pumping_constant e)
+    (H_pumping : forall m : nat, s1 ++ s2 ^ m ++ s3 ∈ e)
+    : PUMPING_spec e s.
+
+Theorem pumping_lemma (e : regex A) (s : list A)
+  (H_in : s ∈ e)
+  (pumping_constant_le : pumping_constant e <= length s)
+  : PUMPING_spec e s.
+Proof.
+  induction H_in as [ | c | s e1 e2 H_INL IHL | s e1 e2 H_INR IHR | s1 s2 e1 e2 H_IN1 IH1 H_IN2 IH2 | e1 | e1 s1 s2 H_IN1 IH1 H_IN2 IH2]; simpl in *.
+  - lia.
+  - lia.
+  - assert (H_le : pumping_constant e1 <= length s) by lia.
+    specialize (IHL H_le). destruct IHL as [s1' s2' s3' ? ? ? ?]. exists s1' s2' s3'.
+    { exact H_split. }
+    { eauto. }
+    { simpl. lia. }
+    { eauto with *. }
+  - assert (H_le : pumping_constant e2 <= length s) by lia.
+    specialize (IHR H_le). destruct IHR as [s1' s2' s3' ? ? ? ?]. exists s1' s2' s3'.
+    { exact H_split. }
+    { eauto. }
+    { simpl. lia. }
+    { eauto with *. }
+  - rewrite length_app in pumping_constant_le.
+    assert (pumping_constant e1 <= length s1 \/ pumping_constant e1 > length s1) as [H_le1 | H_gt1] by lia; [ | assert (pumping_constant e2 <= length s2 \/ pumping_constant e2 > length s2) as [H_le2 | H_gt2] by lia].
+    + specialize (IH1 H_le1). destruct IH1 as [s1' s2' s3' ? ? ? ?]. exists s1' s2' (s3' ++ s2).
+      { rewrite H_split. now repeat rewrite <- app_assoc. }
+      { eauto. }
+      { simpl. lia. }
+      { ii. replace (s1' ++ s2' ^ m ++ s3' ++ s2) with ((s1' ++ s2' ^ m ++ s3') ++ s2) by now repeat rewrite <- app_assoc. econstructor; eauto. }
+    + specialize (IH2 H_le2). destruct IH2 as [s1' s2' s3' ? ? ? ?]. exists (s1 ++ s1') s2' s3'.
+      { rewrite H_split. now repeat rewrite <- app_assoc. }
+      { eauto. }
+      { simpl. rewrite length_app. lia. }
+      { ii. replace ((s1 ++ s1') ++ s2' ^ m  ++ s3') with (s1 ++ (s1' ++ s2' ^ m  ++ s3')) by now repeat rewrite <- app_assoc. econstructor; eauto. }
+    + lia.
+  - pose proof (pumping_constant_ge_1 e1) as H_0_ge_1; lia.
+  - rewrite length_app in pumping_constant_le.
+    destruct s1 as [ | c1 s1']; [ | assert (length (c1 :: s1') < pumping_constant e1 \/ length (c1 :: s1') >= pumping_constant e1) as [H_lt1 | H_ge1] by lia].
+    + simpl. eapply IH2. simpl in *. lia.
+    + exists [] (c1 :: s1') s2.
+      { eauto. }
+      { discriminate. }
+      { simpl in *. lia. }
+      { simpl. ii. eapply pow_star; eauto. }
+    + specialize (IH1 H_ge1). destruct IH1 as [s' s2' s3' ? ? ? ?].
+      exists s' s2' (s3' ++ s2).
+      { rewrite H_split. now repeat rewrite <- app_assoc. }
+      { eauto. }
+      { simpl in *. lia. }
+      { ii. replace (s' ++ s2' ^ m ++ s3' ++ s2) with ((s' ++ s2' ^ m ++ s3') ++ s2) by now repeat rewrite <- app_assoc. eauto with *. }
 Qed.
 
 End LANGUAGE.
